theories/Lambda/ExprDI.v
@@ -164,24 +164,22 @@ Module Type ExprDenote.
 
       Fixpoint uvar_eval tys (ls : list (expr typ func)) {struct ls}
       : option ((hlist typD tys -> exprT tus tvs T) -> exprT tus tvs T) :=
-        match tys as tys
+        match ls , tys as tys
               return option ((hlist typD tys -> exprT tus tvs T) -> exprT tus tvs T)
         with
-          | nil => Some (fun u => u Hnil)
-          | ty :: tys =>
-            match ls with
-              | nil => None
-              | l :: ls =>
-                match exprD' tus tvs ty l with
+          | nil , nil => Some (fun u => u Hnil)
+          | l :: ls , ty :: tys =>
+            match exprD' tus tvs ty l with
+              | None => None
+              | Some val =>
+                match uvar_eval tys ls with
                   | None => None
-                  | Some val =>
-                    match uvar_eval tys ls with
-                      | None => None
-                      | Some result =>
-                        Some (fun u => result (fun z us vs => u (Hcons (val us vs) z) us vs))
-                    end
+                  | Some result =>
+                    Some (fun u => result (fun z us vs => u (Hcons (val us vs) z) us vs))
                 end
             end
+          | nil , _ :: _ => None
+          | _ :: _ , nil => None
         end.
     End uvar_eval.
 
